Refactor path predicates to take the consumed characters

RegexCorrectness/NFA/Transition/Basic.lean
@@ -3,55 +3,55 @@ import RegexCorrectness.NFA.Compile
 
 namespace NFA
 
-inductive stepIn (nfa : NFA) (start : Nat) : (current: Nat) → (input: List Char) → (next: Nat) → (output: List Char) → Prop where
-  | charStep {i j : Nat} {c : Char} {cs : List Char} (h₁ : start ≤ i) (h₂ : i < nfa.nodes.size) (step : j ∈ nfa[i].charStep c) : nfa.stepIn start i (c :: cs) j cs
-  | εStep {i j : Nat} {cs : List Char} (h₁ : start ≤ i) (h₂ : i < nfa.nodes.size) (step : j ∈ nfa[i].εStep) : nfa.stepIn start i cs j cs
+inductive stepIn (nfa : NFA) (start : Nat) : (current next : Nat) → (cs : List Char) → Prop where
+  | charStep {i j : Nat} {c : Char} (h₁ : start ≤ i) (h₂ : i < nfa.nodes.size) (step : j ∈ nfa[i].charStep c) : nfa.stepIn start i j [c]
+  | εStep {i j : Nat} (h₁ : start ≤ i) (h₂ : i < nfa.nodes.size) (step : j ∈ nfa[i].εStep) : nfa.stepIn start i j []
 
-theorem stepIn.h₁ {nfa : NFA} {start : Nat} {i j : Nat} {cs cs' : List Char}
-  (step : nfa.stepIn start i cs j cs') : start ≤ i := by
+theorem stepIn.h₁ {nfa : NFA} {start : Nat} {i j : Nat} {cs : List Char}
+  (step : nfa.stepIn start i j cs) : start ≤ i := by
   cases step with
   | charStep h₁ _ _ => exact h₁
   | εStep h₁ _ _ => exact h₁
 
-theorem stepIn.h₂ {nfa : NFA} {start : Nat} {i j : Nat} {cs cs' : List Char}
-  (step : nfa.stepIn start i cs j cs') : i < nfa.nodes.size := by
+theorem stepIn.h₂ {nfa : NFA} {start : Nat} {i j : Nat} {cs : List Char}
+  (step : nfa.stepIn start i j cs) : i < nfa.nodes.size := by
   cases step with
   | charStep _ h₂ _ => exact h₂
   | εStep _ h₂ _ => exact h₂
 
-theorem stepIn.step {nfa : NFA} {start : Nat} {i j : Nat} {cs cs' : List Char}
-  (step : nfa.stepIn start i cs j cs') :
+theorem stepIn.step {nfa : NFA} {start : Nat} {i j : Nat} {cs : List Char}
+  (step : nfa.stepIn start i j cs) :
   (∃ c, j ∈ (nfa[i]'step.h₂).charStep c) ∨ j ∈ (nfa[i]'step.h₂).εStep := by
   cases step with
   | charStep _ _ step => exact .inl ⟨_, step⟩
   | εStep _ _ step => exact .inr step
 
-theorem le_of_stepIn {start} (step : stepIn nfa start i cs j cs') : start ≤ i := by
+theorem le_of_stepIn {start} (step : stepIn nfa start i j cs) : start ≤ i := by
   cases step with
   | charStep h₁ => exact h₁
   | εStep h₁ => exact h₁
 
-theorem stepIn.lt_right {start} (step : stepIn nfa start i cs j cs') : j < nfa.nodes.size := by
+theorem stepIn.lt_right {start} (step : stepIn nfa start i j cs) : j < nfa.nodes.size := by
   match step.step with
   | .inl ⟨_, step⟩ => exact lt_of_charStep step
   | .inr step => exact lt_of_εStep step
 
 theorem stepIn.castStart' {nfa : NFA} {start start' : Nat}
-  (le : start' ≤ i) (step : stepIn nfa start i cs j cs') :
-  nfa.stepIn start' i cs j cs' := by
+  (le : start' ≤ i) (step : stepIn nfa start i j cs) :
+  nfa.stepIn start' i j cs := by
   cases step with
   | charStep h₁ h₂ step => exact .charStep le h₂ step
   | εStep h₁ h₂ step => exact .εStep le h₂ step
 
 theorem stepIn.castStart {nfa : NFA} {start start' : Nat}
-  (le : start' ≤ start) (step : stepIn nfa start i cs j cs') :
-  nfa.stepIn start' i cs j cs' := step.castStart' (Nat.le_trans le step.h₁)
+  (le : start' ≤ start) (step : stepIn nfa start i j cs) :
+  nfa.stepIn start' i j cs := step.castStart' (Nat.le_trans le step.h₁)
 
 theorem stepIn.cast {nfa nfa' : NFA} {start : Nat}
-  (step : nfa.stepIn start i cs j cs')
+  (step : nfa.stepIn start i j cs)
   (h : i < nfa'.nodes.size)
   (eq : nfa[i]'(step.h₂) = nfa'[i]) :
-  nfa'.stepIn start i cs j cs' := by
+  nfa'.stepIn start i j cs := by
   cases step with
   | charStep h₁ h₂ step =>
     exact .charStep h₁ h (eq ▸ step)
@@ -59,34 +59,35 @@ theorem stepIn.cast {nfa nfa' : NFA} {start : Nat}
     exact .εStep h₁ h (eq ▸ step)
 
 -- Maybe we should recurse from the last as we reason about the last step often
-inductive pathIn (nfa : NFA) (start : Nat) : (index: Nat) → (prefx: List Char) → (next: Nat) → List Char → Prop where
-  | base (h : start ≤ i) (eqi : i = j) (eqs : cs = cs') : nfa.pathIn start i cs j cs'
-  | step {i j k : Nat} {cs cs' cs'' : List Char} (step : nfa.stepIn start i cs j cs') (rest : nfa.pathIn start j cs' k cs'') : nfa.pathIn start i cs k cs''
+inductive pathIn (nfa : NFA) (start : Nat) : (first : Nat) → (last : Nat) → (cs : List Char) → Prop where
+  | base (h : start ≤ i) : nfa.pathIn start i i []
+  | step {i j k : Nat} {cs₁ cs₂ : List Char}
+    (step : nfa.stepIn start i j cs₁) (rest : nfa.pathIn start j k cs₂) : nfa.pathIn start i k (cs₁ ++ cs₂)
 
-theorem le_of_pathIn_left {start} (path : pathIn nfa start i cs j cs') : start ≤ i := by
+theorem le_of_pathIn_left {start} (path : pathIn nfa start i j cs) : start ≤ i := by
   cases path with
   | base h => exact h
   | step step _ => exact le_of_stepIn step
 
-theorem le_of_pathIn_right {start} (path : pathIn nfa start i cs j cs') : start ≤ j := by
+theorem le_of_pathIn_right {start} (path : pathIn nfa start i j cs) : start ≤ j := by
   induction path with
-  | base h eqi => exact eqi ▸ h
+  | base h => exact h
   | step _ _ ih => exact ih
 
 theorem pathIn.castStart {nfa : NFA} {start start' : Nat}
   (le : start' ≤ start)
-  (path : nfa.pathIn start i cs j cs') :
-  nfa.pathIn start' i cs j cs' := by
+  (path : nfa.pathIn start i j cs) :
+  nfa.pathIn start' i j cs := by
   induction path with
-  | base h eqi eqs => exact .base (Nat.le_trans le h) eqi eqs
+  | base h => exact .base (Nat.le_trans le h)
   | step step _ ih => exact .step (step.castStart le) ih
 
 theorem pathIn.cast {nfa nfa' : NFA} (start : Nat)
   (eq : ∀ i, (h₁ : start ≤ i) → (h₂ : i < nfa.nodes.size) → ∃ h' : i < nfa'.nodes.size, nfa[i] = nfa'[i])
-  (path : pathIn nfa start i cs j cs') :
-  pathIn nfa' start i cs j cs' := by
+  (path : pathIn nfa start i j cs) :
+  pathIn nfa' start i j cs := by
   induction path with
-  | base h eqi eqs => exact .base h eqi eqs
+  | base h => exact .base h
   | step step _ ih =>
     let ⟨h, eq⟩ := eq _ step.h₁ step.h₂
     exact .step (step.cast h eq) ih
@@ -94,15 +95,15 @@ theorem pathIn.cast {nfa nfa' : NFA} (start : Nat)
 theorem pathIn.cast' {nfa nfa' : NFA} {start : Nat}
   (assm : i < nfa.nodes.size) (le : nfa.nodes.size ≤ nfa'.nodes.size)
   (eq : ∀ i, (h₁ : start ≤ i) → (h₂ : i < nfa.nodes.size) → nfa[i] = nfa'[i]'(Nat.lt_of_lt_of_le h₂ le))
-  (path : pathIn nfa' start i cs j cs') :
-  pathIn nfa start i cs j cs' := by
+  (path : pathIn nfa' start i j cs) :
+  pathIn nfa start i j cs := by
   induction path with
-  | base h eqi eqs => exact .base h eqi eqs
-  | @step i j k cs cs' cs'' step _ ih =>
+  | base h => exact .base h
+  | @step i j k cs cs' step _ ih =>
     have eq := eq _ step.h₁ assm
     have : j < nfa.nodes.size := by
       cases step with
-      | @charStep _ c _ _ _ step => exact lt_of_charStep (eq.symm ▸ step)
+      | @charStep c _ _ step => exact lt_of_charStep (eq.symm ▸ step)
       | εStep _ _ step => exact lt_of_εStep (eq.symm ▸ step)
     exact .step (step.cast assm eq.symm) (ih this)
 
@@ -113,11 +114,11 @@ theorem pathIn.castLE {nfa : NFA} {start start' i i' : Nat}
     (∃ c, j ∈ nfa[i].charStep c) ∨ j ∈ nfa[i].εStep →
     start ≤ j →
     start' ≤ j)
-  (path : pathIn nfa start i cs i' cs') :
-  pathIn nfa start' i cs i' cs' := by
+  (path : pathIn nfa start i i' cs) :
+  pathIn nfa start' i i' cs := by
   induction path with
-  | base _ eqi eqs => exact .base assm eqi eqs
-  | @step i j k cs cs' cs'' step rest ih =>
+  | base _ => exact .base assm
+  | @step i j k cs cs' step rest ih =>
     have h₂ := step.h₂
     have : start' ≤ j := by
       cases step with
@@ -127,11 +128,11 @@ theorem pathIn.castLE {nfa : NFA} {start start' i i' : Nat}
 
 theorem pathIn.lt_right {nfa : NFA} {start i i' : Nat}
   (assm : i < nfa.nodes.size)
-  (path : pathIn nfa start i cs i' cs') :
+  (path : pathIn nfa start i i' cs) :
   i' < nfa.nodes.size := by
   induction path with
-  | base _ eqi _ => exact eqi ▸ assm
-  | @step i j _ _ _ _ step _ ih =>
+  | base _ => exact assm
+  | @step i j _ _ _ step _ ih =>
     have : j < nfa.nodes.size := by
       cases step with
       | charStep _ _ step => exact lt_of_charStep step
@@ -139,93 +140,109 @@ theorem pathIn.lt_right {nfa : NFA} {start i i' : Nat}
     exact ih this
 
 theorem pathIn.snoc_char {start}
-  (assm₁ : j < nfa.nodes.size) (assm₂ : cs' = c :: cs'')
-  (step : k ∈ nfa[j].charStep c) (path : pathIn nfa start i cs j cs')
-  : pathIn nfa (min start k) i cs k cs'' := by
+  (assm : j < nfa.nodes.size)
+  (step : k ∈ nfa[j].charStep c) (path : pathIn nfa start i j cs)
+  : pathIn nfa (min start k) i k (cs ++ [c]) := by
   induction path with
-  | base h eqi eqs =>
-    subst eqi eqs assm₂
-    exact .step (.charStep (Nat.le_trans (Nat.min_le_left _ _) h) assm₁ step) (.base (Nat.min_le_right _ _) rfl rfl)
-  | step step' rest ih =>
-    have ih := ih assm₁ assm₂ step
-    exact .step (step'.castStart (Nat.min_le_left _ _)) ih
+  | base h =>
+    simp
+    exact .step (.charStep (Nat.le_trans (Nat.min_le_left _ _) h) assm step) (.base (Nat.min_le_right _ _))
+  | @step i j k' cs'' cs''' step' rest ih =>
+    simp
+    have ih := ih assm step
+    exact pathIn.step (step'.castStart (Nat.min_le_left _ _)) ih
 
 theorem pathIn.snoc_ε {start}
   (assm : j < nfa.nodes.size)
-  (step : k ∈ nfa[j].εStep) (path : pathIn nfa start i cs j cs')
-  : pathIn nfa (min start k) i cs k cs' := by
+  (step : k ∈ nfa[j].εStep) (path : pathIn nfa start i j cs)
+  : pathIn nfa (min start k) i k cs := by
   induction path with
-  | base h eqi eqs =>
-    subst eqi eqs
-    exact .step (.εStep (Nat.le_trans (Nat.min_le_left _ _) h) assm step) (.base (Nat.min_le_right _ _) rfl rfl)
+  | base h =>
+    exact .step (.εStep (Nat.le_trans (Nat.min_le_left _ _) h) assm step) (.base (Nat.min_le_right _ _))
   | step step' rest ih =>
     have ih := ih assm step
     exact .step (step'.castStart (Nat.min_le_left _ _)) ih
 
 theorem pathIn.trans {start}
-  (path₁ : pathIn nfa start i cs j cs') (path₂ : pathIn nfa start j cs' k cs'') :
-  pathIn nfa start i cs k cs'' := by
+  (path₁ : pathIn nfa start i j cs) (path₂ : pathIn nfa start j k cs') :
+  pathIn nfa start i k (cs ++ cs') := by
   induction path₁ with
-  | base _ eqi eqs => exact eqi ▸ eqs ▸ path₂
-  | step step _ ih => exact .step step (ih path₂)
+  | base _ => exact path₂
+  | step step _ ih =>
+    simp
+    exact .step step (ih path₂)
 
-def pathToNext (nfa : NFA) (next start i : Nat) (cs cs' : List Char) : Prop :=
-  ∃ (i' : Nat) (cs'' : List Char),
-    nfa.pathIn start i cs i' cs'' ∧
-    nfa.stepIn start i' cs'' next cs'
+def pathToNext (nfa : NFA) (next start i : Nat) (cs : List Char) : Prop :=
+  ∃ (i' : Nat) (pcs scs : List Char),
+    cs = pcs ++ scs ∧
+    nfa.pathIn start i i' pcs ∧
+    nfa.stepIn start i' next scs
 
-theorem le_of_pathToNext {start} (path : pathToNext nfa next start i cs cs') : start ≤ i := by
-  obtain ⟨_, _, path, _⟩ := path
+theorem le_of_pathToNext {start} (path : pathToNext nfa next start i cs) : start ≤ i := by
+  obtain ⟨_, _, _, _, path, _⟩ := path
   exact le_of_pathIn_left path
 
-theorem pathToNext.cons {start} {cs cs' cs'' : List Char}
-  (step : stepIn nfa start i cs j cs') (path : pathToNext nfa next start j cs' cs'') :
-  pathToNext nfa next start i cs cs'' := by
-  obtain ⟨i', cs''', path, step'⟩ := path
-  exact ⟨i', cs''', .step step path, step'⟩
+theorem pathToNext.cons {start} {cs₁ cs₂ : List Char}
+  (step : stepIn nfa start i j cs₁) (path : pathToNext nfa next start j cs₂) :
+  pathToNext nfa next start i (cs₁ ++ cs₂) := by
+  obtain ⟨i', pcs, scs, eqs, path, step'⟩ := path
+  subst eqs
+  cases step with
+  | charStep h₁ h₂ step =>
+    exact ⟨i', _ :: pcs, scs, rfl, .step (.charStep h₁ h₂ step) path, step'⟩
+  | εStep h₁ h₂ step =>
+    exact ⟨i', pcs, scs, rfl, .step (.εStep h₁ h₂ step) path, step'⟩
 
-theorem pathToNext.cast {nfa nfa' : NFA} {next start i : Nat} {cs cs' : List Char}
+theorem pathToNext.cast {nfa nfa' : NFA} {next start i : Nat} {cs : List Char}
   (eq : ∀ i, (h₁ : start ≤ i) → (h₂ : i < nfa.nodes.size) → ∃ h' : i < nfa'.nodes.size, nfa[i] = nfa'[i])
-  (path : pathToNext nfa next start i cs cs') :
-  pathToNext nfa' next start i cs cs' := by
-  obtain ⟨i', cs'', path, step⟩ := path
+  (path : pathToNext nfa next start i cs) :
+  pathToNext nfa' next start i cs := by
+  obtain ⟨i', pcs, scs, eqs, path, step⟩ := path
   obtain ⟨h', eq'⟩ := eq _ (le_of_pathIn_right path) step.h₂
-  exact ⟨i', cs'', pathIn.cast start eq path, step.cast h' eq'⟩
+  exact ⟨i', pcs, scs, eqs, pathIn.cast start eq path, step.cast h' eq'⟩
 
 theorem pathToNext.cast' {nfa nfa' : NFA} {start : Nat}
   (assm : i < nfa.nodes.size) (le : nfa.nodes.size ≤ nfa'.nodes.size)
   (eq : ∀ i, (h₁ : start ≤ i) → (h₂ : i < nfa.nodes.size) → nfa[i] = nfa'[i]'(Nat.lt_of_lt_of_le h₂ le))
-  (path : pathToNext nfa' next start i cs cs') :
-  pathToNext nfa next start i cs cs' := by
-  obtain ⟨i', cs'', path, step⟩ := path
+  (path : pathToNext nfa' next start i cs) :
+  pathToNext nfa next start i cs := by
+  obtain ⟨i', pcs, scs, eqs, path, step⟩ := path
   have path' := path.cast' assm le eq
   have lt : i' < nfa.nodes.size := path'.lt_right assm
-  exact ⟨i', cs'', path', step.cast lt (eq i' step.h₁ lt).symm⟩
+  exact ⟨i', pcs, scs, eqs, path', step.cast lt (eq i' step.h₁ lt).symm⟩
 
-theorem pathToNext.castStart {nfa : NFA} {start start' : Nat} {i : Nat} {cs cs' : List Char}
-  (le : start' ≤ start) (path : pathToNext nfa next start i cs cs') :
-  pathToNext nfa next start' i cs cs' := by
-  obtain ⟨i', cs'', path, step⟩ := path
-  exact ⟨i', cs'', path.castStart le, step.castStart le⟩
+theorem pathToNext.castStart {nfa : NFA} {start start' : Nat} {i : Nat} {cs : List Char}
+  (le : start' ≤ start) (path : pathToNext nfa next start i cs) :
+  pathToNext nfa next start' i cs := by
+  obtain ⟨i', pcs, scs, eqs, path, step⟩ := path
+  exact ⟨i', pcs, scs, eqs, path.castStart le, step.castStart le⟩
 
-theorem pathToNext.castLE {nfa : NFA} {next start start' i : Nat} {cs cs' : List Char}
+theorem pathToNext.castLE {nfa : NFA} {next start start' i : Nat} {cs : List Char}
   (assm : start' ≤ i)
   (inBounds : ∀ i j, (h₁ : start' ≤ i) →
     (h₂ : i < nfa.nodes.size) →
     (∃ c, j ∈ nfa[i].charStep c) ∨ j ∈ nfa[i].εStep →
     start ≤ j →
     start' ≤ j)
-  (path : pathToNext nfa next start i cs cs') :
-  pathToNext nfa next start' i cs cs' := by
-  obtain ⟨i', cs'', path, step⟩ := path
+  (path : pathToNext nfa next start i cs) :
+  pathToNext nfa next start' i cs := by
+  obtain ⟨i', pcs, scs, eqs, path, step⟩ := path
   have path' := path.castLE assm inBounds
-  exact ⟨i', cs'', path', step.castStart' (le_of_pathIn_right path')⟩
+  exact ⟨i', pcs, scs, eqs, path', step.castStart' (le_of_pathIn_right path')⟩
 
-theorem pathToNext.trans {nfa : NFA} {start : Nat} {cs cs' cs'' : List Char}
-  (path₁ : pathToNext nfa j start i cs cs') (path₂ : pathToNext nfa k start j cs' cs'') :
-  pathToNext nfa k start i cs cs'' := by
-  obtain ⟨i', cs''', path₁, step₁⟩ := path₁
-  obtain ⟨j', cs'''', path₂, step₂⟩ := path₂
-  exact ⟨j', cs'''', path₁.trans (.step step₁ path₂), step₂⟩
+theorem pathToNext.trans {nfa : NFA} {start : Nat} {cs cs' : List Char}
+  (path₁ : pathToNext nfa j start i cs) (path₂ : pathToNext nfa k start j cs') :
+  pathToNext nfa k start i (cs ++ cs') := by
+  obtain ⟨i₁, pcs₁, scs₁, eqs₁, path₁, step₁⟩ := path₁
+  obtain ⟨i₂, pcs₂, scs₂, eqs₂, path₂, step₂⟩ := path₂
+  exact ⟨i₂, pcs₁ ++ (scs₁ ++ pcs₂), scs₂, by simp [eqs₁, eqs₂], path₁.trans (.step step₁ path₂), step₂⟩
+
+theorem pathIn_of_pathToNext {nfa : NFA} {start : Nat}
+  (path : pathToNext nfa next start i cs) :
+  pathIn nfa (min start next) i next cs := by
+  obtain ⟨i', pcs, scs, eqs, path, step⟩ := path
+  cases step with
+  | charStep h₁ h₂ step => exact eqs ▸ path.snoc_char h₂ step
+  | εStep h₁ h₂ step => simp [eqs, path.snoc_ε h₂ step]
 
 end NFA
