RegexCorrectness/NFA/VM/Correctness2.lean
@@ -3,31 +3,109 @@ import RegexCorrectness.NFA.Transition
 
 namespace NFA
 
-theorem pathIn_of_reaches {nfa : NFA} {i : Fin nfa.nodes.size} {m r : List Char}
+theorem pathIn_of_reaches {nfa : NFA} {i : Fin nfa.nodes.size} {m : List Char}
   (h : nfa.reaches i m) :
-  nfa.pathIn 0 nfa.start (m ++ r) i r := by
-  induction h generalizing r with
+  nfa.pathIn 0 nfa.start i m := by
+  induction h with
   | nil cls => simp [pathIn_iff_εClosure.mpr cls]
   | @snoc i j k c m _ step cls ih =>
-    simp
     simp [charStep] at step
-    have ih' : nfa.pathIn (min 0 j) nfa.start (m ++ c :: r) j r :=
-      ih.snoc_char i.isLt rfl step
+    have ih' : nfa.pathIn (min 0 j) nfa.start j (m ++ [c]) :=
+      ih.snoc_char i.isLt step
     simp at ih'
-    exact ih'.trans (pathIn_iff_εClosure.mpr cls)
+    have := ih'.trans (pathIn_iff_εClosure.mpr cls)
+    simp at this
+    exact this
+
+theorem stepIn.nil_or_singleton {start} (h : stepIn nfa start i j cs) :
+  cs = [] ∨ ∃ c, cs = [c] := by
+  cases h with
+  | εStep => exact .inl rfl
+  | charStep => exact .inr ⟨_, rfl⟩
+
+theorem stepIn.nil_of_snoc {start} (h : stepIn nfa start i j (cs ++ [c])) :
+  cs = [] := by
+  generalize h' : cs ++ [c] = cs' at h
+  cases h with
+  | εStep => simp at h'
+  | charStep =>
+    cases cs with
+    | nil => rfl
+    | cons _ _ =>
+      have := congrArg List.length h'
+      simp at this
+
+theorem pathIn.of_snoc_char {start}
+  (path : pathIn nfa start i l (cs ++ [c])) :
+  ∃ j k, pathIn nfa start i j cs ∧ k ∈ nfa.charStep j c ∧ l ∈ nfa.εClosure k := by
+  generalize h : cs ++ [c] = cs' at path
+  induction path generalizing cs with
+  | base _ => simp at h
+  | @step i j k cs₁ cs₂ step rest ih =>
+    match snoc_eq_append h with
+    | .inl ⟨h₁, h₂⟩ =>
+      simp [h₁, h₂] at step rest
+      have := step.nil_of_snoc
+      simp [this] at *
+      cases step with
+      | charStep le _ step =>
+        exact ⟨i, .base le, j, charStep_of_charStep step, εClosure_of_pathIn rest⟩
+    | .inr ⟨cs₂', h₁, h₂⟩ =>
+      have ⟨j', k', path', step', cls⟩ := ih h₂.symm
+      exact ⟨j', k', h₁ ▸ .step step path', step', cls⟩
+where
+  snoc_eq_append {cs₁ cs₂ cs₃ : List Char} {c : Char} (h : cs₁ ++ [c] = cs₂ ++ cs₃) :
+    (cs₂ = cs₁ ++ [c] ∧ cs₃ = []) ∨ (∃ cs₃', cs₁ = cs₂ ++ cs₃' ∧ cs₃ = cs₃' ++ [c]) := by
+    cases cs₃ using List.list_reverse_induction with
+    | base =>
+      simp at h
+      exact .inl ⟨h.symm, rfl⟩
+    | ind cs₃ c' =>
+      have : c = c' ∧ cs₁ = cs₂ ++ cs₃ := by
+        have h₁ := congrArg List.reverse h
+        simp at h₁
+        have h₂ := congrArg List.reverse h₁.right
+        simp at h₂
+        exact ⟨h₁.left, h₂⟩
+      simp [this]
+
+theorem reaches_of_pathIn {nfa : NFA} {i : Fin nfa.nodes.size} {m : List Char}
+  (h : nfa.pathIn 0 nfa.start i m) :
+  nfa.reaches i m := by
+  induction m using List.list_reverse_induction generalizing i with
+  | base => exact .nil (pathIn_iff_εClosure.mp h)
+  | ind m c ih =>
+    have ⟨j, k, path, step, cls⟩ := pathIn.of_snoc_char h
+    let j' : Fin nfa.nodes.size := ⟨j, path.lt_right nfa.start.isLt⟩
+    have prev := ih (i := j') path
+    exact .snoc prev step cls
+
+theorem reaches_iff_pathIn {nfa : NFA} {i : Fin nfa.nodes.size} {m : List Char} :
+  nfa.reaches i m ↔ nfa.pathIn 0 nfa.start i m := ⟨pathIn_of_reaches, reaches_of_pathIn⟩
 
 theorem matches_of_reaches (eq : compile r = nfa)
   (h₁ : nfa.reaches i cs.data) (h₂ : nfa[i] = .done) :
   r.matches cs := by
   have hi : i.val = 0 := (done_iff_zero_compile eq i).mp h₂
-  have : nfa.pathIn 0 nfa.start (cs.data ++ []) i [] := pathIn_of_reaches (r := []) h₁
+  have : nfa.pathIn 0 nfa.start i cs.data := pathIn_of_reaches h₁
   simp at this
   have := pathToNext_of_compile_of_pathIn eq (hi ▸ this)
-  have ⟨cs', eqs, m⟩ := (matches_prefix_iff_pathToNext eq).mpr this
-  have := String.ext_iff.mp eqs
+  exact (matches_iff_pathToNext eq).mpr this
+
+theorem reaches_of_matches (eq : compile r = nfa)
+  (m : r.matches cs) :
+  ∃ i, nfa.reaches i cs.data ∧ nfa[i] = .done := by
+  have := (matches_iff_pathToNext eq).mp m
+  have := pathIn_of_pathToNext this
   simp at this
-  have := String.ext this
-  exact this ▸ m
+  let i' : Fin nfa.nodes.size := ⟨0, lt_zero_size_compile eq⟩
+  have := reaches_of_pathIn (i := i') this
+  have hdone := (done_iff_zero_compile eq i').mpr rfl
+  exact ⟨i', this, hdone⟩
+
+theorem matches_iff_reaches (eq : compile r = nfa) :
+  r.matches cs ↔ ∃ i, nfa.reaches i cs.data ∧ nfa[i] = .done :=
+  ⟨reaches_of_matches eq, fun ⟨_, h₁, h₂⟩ => matches_of_reaches eq h₁ h₂⟩
 
 theorem matches_of_captureNext
   (eq : compile re = nfa)
